Halicore_Type_Meaning.thy: completely revised and updated

isa/Halicore_Type_Meaning.thy
@@ -1,60 +1,154 @@
 header {* Meaning function for type expressions *}
 
 theory Halicore_Type_Meaning
-imports Halicore Halicore_Type_Deep
+imports
+  Halicore_Type_Deep
+  Defl_Lib
+  "~~/src/HOL/Library/Countable"
+  "~~/src/HOL/HOLCF/Library/HOL_Cpo"
 begin
 
-definition Uapp :: "U \<rightarrow> U \<rightarrow> U"
-  where "Uapp = (\<Lambda> (Ufun\<cdot>f). f)"
+subsection {* Domain definition for Core values *}
 
-lemma Uapp_Ufun [simp]: "Uapp\<cdot>(Ufun\<cdot>f) = f"
-unfolding Uapp_def
-by (cases "f = \<bottom>", simp_all)
+text {* We must first show that type @{text ty} is countable. *}
 
-primrec nat_append :: "'a::type list \<Rightarrow> (nat \<Rightarrow> 'a) \<Rightarrow> nat \<Rightarrow> 'a"
-  where "nat_append [] f = f"
-  | "nat_append (x # xs) f = nat_case x (nat_append xs f)"
+instance kind :: countable
+  by countable_datatype
+
+instance base :: countable
+  by countable_datatype
+
+instance visibility :: countable
+  by countable_datatype
+
+instance ty :: countable
+  by countable_datatype
+
+domain V
+  = Vint (lazy "int")
+  | Vcon (lazy "nat") (lazy "V list")
+  | Vfun (lazy "V \<rightarrow> V")
+  | Vtfun (lazy "ty discr \<rightarrow> V")
+  | Wrong
+
+subsection {* Deflation model of types *}
+
+domain U = Udefl (unUdefl :: "V defl") | Ufun (Uapp :: "U \<rightarrow> U")
+
+definition TyFun_denote :: "U"
+  where "TyFun_denote = Ufun\<cdot>(\<Lambda> a. Ufun\<cdot>(\<Lambda> b.
+    Udefl\<cdot>(defl_fun2 (\<Lambda>(up\<cdot>f). Vfun\<cdot>f) (\<Lambda>(Vfun\<cdot>f). up\<cdot>f)
+      (\<Lambda> d e. u_map\<cdot>(cfun_map\<cdot>d\<cdot>e))\<cdot>(unUdefl\<cdot>a)\<cdot>(unUdefl\<cdot>b))))"
 
 primrec base_denote :: "base \<Rightarrow> U"
-  where "base_denote TyFun = to_U\<cdot>Tfun"
+  where "base_denote TyFun = TyFun_denote"
   | "base_denote TyInt = \<bottom>"
   | "base_denote TyChar = \<bottom>"
 
-consts Tdata' :: "string \<rightarrow> T list list \<rightarrow> T"
+subsubsection {* Datatypes *}
 
-definition Uforall :: "(U \<rightarrow> U) \<rightarrow> U"
-  where "Uforall = (\<Lambda> f. Udefl\<cdot>(T_abs\<cdot>(defl_fun1 (fup\<cdot>Vtfun) (V_case\<cdot>\<bottom>\<cdot>\<bottom>\<cdot>\<bottom>\<cdot>up\<cdot>\<bottom>) u_map\<cdot>(pi_defl\<cdot>ID_defl\<cdot>(\<Lambda> u. T_rep\<cdot>(of_U\<cdot>(f\<cdot>u)))))))"
+definition Nil_defl :: "'a list u defl"
+  where "Nil_defl = defl_principal (Abs_fin_defl
+    (\<Lambda>(up\<cdot>xs). case xs of [] \<Rightarrow> up\<cdot>[] | y # ys \<Rightarrow> \<bottom>))"
 
-primrec ty_denote :: "(nat \<Rightarrow> U) \<Rightarrow> ty \<Rightarrow> U"
-  and cons_denote :: "(nat \<Rightarrow> U) \<Rightarrow> ty list list \<Rightarrow> T list list"
-  and args_denote :: "(nat \<Rightarrow> U) \<Rightarrow> ty list \<Rightarrow> T list"
-where ty_denote_TyVar:
-    "ty_denote \<sigma> (TyVar n) = \<sigma> n"
-  | ty_denote_TyBase:
-    "ty_denote \<sigma> (TyBase b) = base_denote b"
-  | ty_denote_TyApp:
-    "ty_denote \<sigma> (TyApp t1 t2) =
-      Uapp\<cdot>(ty_denote \<sigma> t1)\<cdot>(ty_denote \<sigma> t2)"
-  | ty_denote_TyAll:
-    "ty_denote \<sigma> (TyAll k t) =
-      Uforall\<cdot>(\<Lambda> u. ty_denote (nat_case u \<sigma>) t)"
-  | ty_denote_TyLam:
-    "ty_denote \<sigma> (TyLam k t) =
-      Ufun\<cdot>(\<Lambda> x. ty_denote (nat_case x \<sigma>) t)" (* FIXME: don't ignore k *)
-  | ty_denote_TyFix:
-    "ty_denote \<sigma> (TyFix k t) = (\<mu> x. ty_denote (nat_case x \<sigma>) t)"
-  | ty_denote_TyRec:
-    "ty_denote \<sigma> (TyRec k t) = (\<mu> x. ty_denote (nat_case x \<sigma>) t)"
-  | ty_denote_TyData:
-    "ty_denote \<sigma> (TyData s tss) = to_U\<cdot>(Tdata'\<cdot>s\<cdot>(cons_denote \<sigma> tss))"
-  | cons_denote_Nil:
-    "cons_denote \<sigma> [] = []"
-  | cons_denote_Cons:
-    "cons_denote \<sigma> (ts # tss) = args_denote \<sigma> ts # cons_denote \<sigma> tss"
-  | args_denote_Nil:
-    "args_denote \<sigma> [] = []"
-  | args_denote_Cons:
-    "args_denote \<sigma> (t # ts) = of_U\<cdot>(ty_denote \<sigma> t) # args_denote \<sigma> ts"
+lemma cast_Nil_defl:
+  "cast\<cdot>Nil_defl = (\<Lambda>(up\<cdot>xs). case xs of [] \<Rightarrow> up\<cdot>[] | y # ys \<Rightarrow> \<bottom>)"
+unfolding Nil_defl_def
+apply (subst cast_defl_principal)
+apply (rule Abs_fin_defl_inverse, simp)
+apply default
+apply (case_tac x, simp, rename_tac xs, case_tac xs, simp, simp)
+apply (case_tac x, simp, rename_tac xs, case_tac xs, simp, simp)
+apply (rule finite_range_imp_finite_fixes)
+apply (rule rev_finite_subset [where B="{\<bottom>, up\<cdot>[]}"], simp)
+apply (clarsimp, rename_tac y, case_tac y, simp, case_tac x, simp, simp)
+done
+
+definition Cons_defl :: "'a u defl \<rightarrow> 'a list u defl \<rightarrow> 'a list u defl"
+  where "Cons_defl = defl_fun2
+    (\<Lambda>(:up\<cdot>x, up\<cdot>xs:). up\<cdot>(x # xs))
+    (\<Lambda>(up\<cdot>ys). case ys of [] \<Rightarrow> \<bottom> | x # xs \<Rightarrow> (:up\<cdot>x, up\<cdot>xs:))
+    sprod_map"
+
+lemma cast_Cons_defl:
+  "cast\<cdot>(Cons_defl\<cdot>a\<cdot>b) = (\<Lambda>(:up\<cdot>x, up\<cdot>xs:). up\<cdot>(x # xs))
+    oo sprod_map\<cdot>(cast\<cdot>a)\<cdot>(cast\<cdot>b) oo
+    (\<Lambda>(up\<cdot>ys). case ys of [] \<Rightarrow> \<bottom> | x # xs \<Rightarrow> (:up\<cdot>x, up\<cdot>xs:))"
+unfolding Cons_defl_def
+apply (rule cast_defl_fun2)
+apply (rule ep_pair.intro)
+apply (rename_tac p, case_tac p, simp)
+apply (case_tac x, simp, case_tac y, simp, simp)
+apply (case_tac y, simp, case_tac x, simp, simp)
+apply (erule (1) finite_deflation_sprod_map)
+done
+
+fixrec defls :: "'a defl list \<rightarrow> 'a list u defl"
+  where "defls\<cdot>[] = Nil_defl"
+  | "defls\<cdot>(d # ds) = Cons_defl\<cdot>(defl_fun1 ID ID u_map\<cdot>d)\<cdot>(defls\<cdot>ds)"
+
+lemma cont2cont_nat_case_simple [simp, cont2cont]:
+  assumes "cont (\<lambda>x. f1 x)"
+  assumes "\<And>n'. cont (\<lambda>x. f2 x n')"
+  shows "cont (\<lambda>x. case n of 0 \<Rightarrow> f1 x | Suc n' \<Rightarrow> f2 x n')"
+using assms by (cases n) auto -- "TODO: move to library"
+
+fixrec nth_defls :: "V defl list list \<rightarrow> nat \<rightarrow> V list u defl"
+  where "nth_defls\<cdot>(ds # dss)\<cdot>n =
+    (case n of 0 \<Rightarrow> defls\<cdot>ds | Suc n' \<Rightarrow> nth_defls\<cdot>dss\<cdot>n')"
+
+lemma nth_defls_Nil: "nth_defls\<cdot>[]\<cdot>n = \<bottom>"
+by fixrec_simp
+
+lemma nth_defls_eq:
+  "nth_defls\<cdot>dss\<cdot>n = (if n < length dss then defls\<cdot>(dss ! n) else \<bottom>)"
+by (induct dss arbitrary: n, simp add: nth_defls_Nil, simp split: nat.split)
+
+definition datadefl :: "V defl list list \<rightarrow> V defl"
+  where "datadefl = (\<Lambda> xs. defl_fun1
+    (\<Lambda>(:up\<cdot>n, up\<cdot>vs:). Vcon\<cdot>n\<cdot>vs) (\<Lambda>(Vcon\<cdot>n\<cdot>vs). (:up\<cdot>n, up\<cdot>vs:)) ID\<cdot>
+  (sprod_of_prod_defl\<cdot>(sig_defl\<cdot>ID_defl\<cdot>(\<Lambda>(up\<cdot>n). nth_defls\<cdot>xs\<cdot>n))))"
+
+lemma cast_datadefl:
+  "cast\<cdot>(datadefl\<cdot>xs) = (\<Lambda>(Vcon\<cdot>s\<cdot>vs). ssplit\<cdot>(\<Lambda> (up\<cdot>s).
+    fup\<cdot>(Vcon\<cdot>s))\<cdot>(:up\<cdot>s, cast\<cdot>(nth_defls\<cdot>xs\<cdot>s)\<cdot>(up\<cdot>vs):))"
+apply (simp add: datadefl_def)
+apply (subst cast_defl_fun1)
+apply (rule ep_pair.intro)
+apply (case_tac x, simp, rename_tac a b)
+apply (case_tac a, simp, case_tac b, simp, simp)
+apply (case_tac y, simp, simp, simp, simp, simp, simp)
+apply simp
+apply (simp add: cast_sprod_of_prod_defl cast_sig_defl)
+apply (rule cfun_eqI, simp)
+apply (case_tac x, simp_all add: eta_cfun)
+done
+
+subsubsection {* Forall-types *}
+
+definition Uforall :: "kind \<Rightarrow> (ty discr \<rightarrow> V defl) \<rightarrow> V defl"
+  where "Uforall k = (\<Lambda> h. defl_fun1 (fup\<cdot>Vtfun) (V_case\<cdot>\<bottom>\<cdot>\<bottom>\<cdot>\<bottom>\<cdot>up\<cdot>\<bottom>) u_map\<cdot>
+    (defl_fun1 decode_cfun encode_cfun ID\<cdot>(strict_pi_defl\<cdot>ID_defl\<cdot>
+      (\<Lambda>(up\<cdot>x). if has_kind [] (undiscr x) k then h\<cdot>x else \<bottom>))))"
+
+lemma cast_Uforall:
+  "cast\<cdot>(Uforall k\<cdot>h) = fup\<cdot>Vtfun oo u_map\<cdot>(\<Lambda> f x. if has_kind [] (undiscr x) k
+    then cast\<cdot>(h\<cdot>x)\<cdot>(f\<cdot>x) else \<bottom>) oo V_case\<cdot>\<bottom>\<cdot>\<bottom>\<cdot>\<bottom>\<cdot>up\<cdot>\<bottom>"
+unfolding Uforall_def
+apply simp
+apply (subst cast_defl_fun1)
+apply (rule ep_pair.intro)
+apply (case_tac x, simp, simp)
+apply (case_tac y, simp, simp, simp, simp, simp, simp)
+apply (erule finite_deflation_u_map)
+apply (intro cfun_arg_cong cfun_fun_cong)
+apply (subst cast_defl_fun1, simp add: ep_pair_def, simp)
+apply (subst cast_strict_pi_defl)
+apply (simp add: decode_cfun_def encode_cfun_def cfun_eq_iff)
+done
+
+lemma LAM_eqI: "(\<And>x. f x = g x) \<Longrightarrow> (\<Lambda> x. f x) = (\<Lambda> y. g y)"
+by simp (* TODO: put in library *)
 
 lemma cont2cont_nat_case [simp, cont2cont]:
   assumes f: "cont f" and g: "cont g"
@@ -64,120 +158,148 @@ apply (case_tac n, simp_all add: f)
 apply (rule cont_compose [OF cont_fun g])
 done
 
-lemma
-  shows cont_ty_denote: "cont (\<lambda>\<sigma>. ty_denote \<sigma> t)"
-  and cont_cons_denote: "cont (\<lambda>\<sigma>. cons_denote \<sigma> tss)"
-  and cont_args_denote: "cont (\<lambda>\<sigma>. args_denote \<sigma> ts)"
-apply (induct t and tss and ts)
-txt "TyVar"
-apply (simp, rule cont_fun)
-txt "TyBase"
-apply simp
-txt "TyApp"
-apply simp
-txt "TyAll"
-apply simp
-apply (intro cont2cont)
-apply (erule cont_compose, simp)
-txt "TyLam"
-apply simp
-apply (intro cont2cont)
-apply (erule cont_compose, simp)
-txt "TyFix"
-apply simp
-apply (intro cont2cont)
-apply (erule cont_compose, simp)
-txt "TyRec"
-apply simp
-apply (intro cont2cont)
-apply (erule cont_compose, simp)
+definition ty_denote' :: "(nat \<Rightarrow> U) \<rightarrow> ty discr \<rightarrow> U"
+  where "ty_denote' = (\<mu> ty_denote'. \<Lambda> \<sigma> t.
+    case undiscr t of TyVar n \<Rightarrow> \<sigma> n
+    | TyBase b \<Rightarrow> base_denote b
+    | TyApp t1 t2 \<Rightarrow> Uapp\<cdot>(ty_denote'\<cdot>\<sigma>\<cdot>(Discr t1))\<cdot>(ty_denote'\<cdot>\<sigma>\<cdot>(Discr t2))
+    | TyAll k t \<Rightarrow>
+      Udefl\<cdot>(Uforall k\<cdot>(\<Lambda> u. unUdefl\<cdot>
+        (ty_denote'\<cdot>(nat_case (ty_denote'\<cdot>\<bottom>\<cdot>u) \<sigma>)\<cdot>(Discr t))))
+    | TyLam k t \<Rightarrow> Ufun\<cdot>(\<Lambda> x. ty_denote'\<cdot>(nat_case x \<sigma>)\<cdot>(Discr t))
+    | TyFix v k t \<Rightarrow> (\<mu> x. ty_denote'\<cdot>(nat_case x \<sigma>)\<cdot>(Discr t))
+    | TyData tss \<Rightarrow>
+      Udefl\<cdot>(datadefl\<cdot>(map (map (\<lambda>t. unUdefl\<cdot>(ty_denote'\<cdot>\<sigma>\<cdot>(Discr t)))) tss)))"
 
-apply simp (* TyData *)
-apply simp (* [] *)
-apply simp (* ts # tss *)
-apply simp (* [] *)
-apply simp (* t # ts *)
+lemma cont2cont_map_simple [simp, cont2cont]:
+  fixes f :: "'a::cpo \<Rightarrow> 'b::type \<Rightarrow> 'c::cpo"
+  assumes f: "\<And>y. cont (\<lambda>x. f x y)"
+  shows "cont (\<lambda>x. map (\<lambda>y. f x y) xs)"
+  by (induct xs, simp_all add: f)
+
+lemma ty_denote'_unfold:
+  "ty_denote'\<cdot>\<sigma>\<cdot>t =
+    (case undiscr t of TyVar n \<Rightarrow> \<sigma> n
+    | TyBase b \<Rightarrow> base_denote b
+    | TyApp t1 t2 \<Rightarrow> Uapp\<cdot>(ty_denote'\<cdot>\<sigma>\<cdot>(Discr t1))\<cdot>(ty_denote'\<cdot>\<sigma>\<cdot>(Discr t2))
+    | TyAll k t \<Rightarrow>
+      Udefl\<cdot>(Uforall k\<cdot>(\<Lambda> u. unUdefl\<cdot>
+        (ty_denote'\<cdot>(nat_case (ty_denote'\<cdot>\<bottom>\<cdot>u) \<sigma>)\<cdot>(Discr t))))
+    | TyLam k t \<Rightarrow> Ufun\<cdot>(\<Lambda> x. ty_denote'\<cdot>(nat_case x \<sigma>)\<cdot>(Discr t))
+    | TyFix v k t \<Rightarrow> (\<mu> x. ty_denote'\<cdot>(nat_case x \<sigma>)\<cdot>(Discr t))
+    | TyData tss \<Rightarrow>
+      Udefl\<cdot>(datadefl\<cdot>(map (map (\<lambda>t. unUdefl\<cdot>(ty_denote'\<cdot>\<sigma>\<cdot>(Discr t)))) tss)))"
+apply (subst def_cont_fix_eq [OF ty_denote'_def [THEN eq_reflection]])
+apply (rule cont2cont_LAM')
+apply (rule cont2cont_LAM_discrete)
+apply (case_tac "undiscr t", simp_all)
+apply (simp add: cont2cont_fun)
+apply (subst beta_cfun)
+apply (rule cont2cont_LAM_discrete)
+apply (case_tac "undiscr t", simp_all)
+apply (rule cont2cont_fun, rule cont_id)
 done
 
+definition ty_denote :: "(nat \<Rightarrow> U) \<Rightarrow> ty \<Rightarrow> U"
+  where "ty_denote \<sigma> t = ty_denote'\<cdot>\<sigma>\<cdot>(Discr t)"
+
+lemma ty_denote_simps [simp]:
+  "ty_denote \<sigma> (TyVar n) = \<sigma> n"
+  "ty_denote \<sigma> (TyBase b) = base_denote b"
+  "ty_denote \<sigma> (TyApp t1 t2) = Uapp\<cdot>(ty_denote \<sigma> t1)\<cdot>(ty_denote \<sigma> t2)"
+  "ty_denote \<sigma> (TyAll k t) =
+      Udefl\<cdot>(Uforall k\<cdot>(\<Lambda> u. unUdefl\<cdot>
+        (ty_denote (nat_case (ty_denote \<bottom> (undiscr u)) \<sigma>) t)))"
+  "ty_denote \<sigma> (TyLam k t) = Ufun\<cdot>(\<Lambda> x. ty_denote (nat_case x \<sigma>) t)"
+  "ty_denote \<sigma> (TyFix v k t) = (\<mu> x. ty_denote (nat_case x \<sigma>) t)"
+  "ty_denote \<sigma> (TyData tss) =
+      Udefl\<cdot>(datadefl\<cdot>(map (map (\<lambda>t. unUdefl\<cdot>(ty_denote \<sigma> t))) tss))"
+unfolding ty_denote_def
+by (subst ty_denote'_unfold, simp)+
+
+lemma cont_ty_denote: "cont (\<lambda>\<sigma>. ty_denote \<sigma> t)"
+  unfolding ty_denote_def by simp
+
 declare cont_ty_denote [THEN cont_compose, simp, cont2cont]
+
+subsection {* Convertibility relation preserves meaning *}
+
+lemma ty_induct:
+  assumes TyVar: "\<And>n. P (TyVar n)"
+  assumes TyBase: "\<And>b. P (TyBase b)"
+  assumes TyApp: "\<And>t1 t2. \<lbrakk>P t1; P t2\<rbrakk> \<Longrightarrow> P (TyApp t1 t2)"
+  assumes TyAll: "\<And>k t. P t \<Longrightarrow> P (TyAll k t)"
+  assumes TyLam: "\<And>k t. P t \<Longrightarrow> P (TyLam k t)"
+  assumes TyFix: "\<And>v k t. P t \<Longrightarrow> P (TyFix v k t)"
+  assumes TyData: "\<And>tss. list_all (list_all P) tss \<Longrightarrow> P (TyData tss)"
+  shows "P t"
+apply (induct t)
+apply (rule TyVar)
+apply (rule TyBase)
+apply (erule (1) TyApp)
+apply (erule TyAll)
+apply (erule TyLam)
+apply (erule TyFix)
+apply (erule TyData)
+apply (simp, simp, simp, simp)
+done
 
 lemma nat_case_substVar [simp]:
   "nat_case u (substVar \<sigma> i x) = substVar (nat_case u \<sigma>) (Suc i) x"
 by (rule ext, rename_tac n, case_tac n, simp_all)
 
-lemma
-  shows ty_denote_ty_lift:
-    "ty_denote (substVar \<sigma> i y) (ty_lift i t) = ty_denote \<sigma> t"
-  and cons_denote_cons_lift:
-    "cons_denote (substVar \<sigma> i y) (cons_lift i tss) = cons_denote \<sigma> tss"
-  and args_denote_args_lift:
-    "args_denote (substVar \<sigma> i y) (args_lift i ts) = args_denote \<sigma> ts"
-by (induct t and tss and ts arbitrary: \<sigma> i and \<sigma> i and \<sigma> i)
-  simp_all
+lemma ty_denote_ty_lift:
+  "ty_denote (substVar \<sigma> i y) (ty_lift i t) = ty_denote \<sigma> t"
+apply (induct t arbitrary: \<sigma> i rule: ty_induct)
+apply simp_all
+apply (simp add: cons_lift_conv_map args_lift_conv_map o_def)
+apply (simp add: list_all_iff cong: map_cong)
+done
 
 lemma substVar_0: "substVar \<sigma> 0 x = nat_case x \<sigma>"
 by (rule ext, rename_tac n, case_tac n, simp_all)
 
-lemma LAM_eqI: "(\<And>x. f x = g x) \<Longrightarrow> (\<Lambda> x. f x) = (\<Lambda> y. g y)"
-by simp (* TODO: put in library *)
-
-lemma
-  shows ty_denote_ty_subst:
-    "ty_denote \<sigma> (ty_subst i t x) =
-     ty_denote (substVar \<sigma> i (ty_denote \<sigma> x)) t"
-  and cons_denote_cons_subst:
-    "cons_denote \<sigma> (cons_subst i tss x) =
-     cons_denote (substVar \<sigma> i (ty_denote \<sigma> x)) tss"
-  and args_denote_args_subst:
-    "args_denote \<sigma> (args_subst i ts x) =
-     args_denote (substVar \<sigma> i (ty_denote \<sigma> x)) ts"
-apply (induct t and tss and ts arbitrary: \<sigma> i x and \<sigma> i x and \<sigma> i x)
+lemma ty_denote_ty_subst:
+  "ty_denote \<sigma> (ty_subst i t x) =
+    ty_denote (substVar \<sigma> i (ty_denote \<sigma> x)) t"
+apply (induct t arbitrary: \<sigma> i x rule: ty_induct)
 apply (simp add: substVar_def) (* TyVar *)
 apply simp (* TyBase *)
 apply simp (* TyApp *)
-txt "TyAll"
-apply (simp add: ty_denote_ty_lift [where i=0, unfolded substVar_0])
-txt "TyLam"
-apply (simp add: ty_denote_ty_lift [where i=0, unfolded substVar_0])
-txt "TyFix"
-apply (simp add: ty_denote_ty_lift [where i=0, unfolded substVar_0])
-txt "TyRec"
-apply (simp add: ty_denote_ty_lift [where i=0, unfolded substVar_0])
-apply simp (* TyData *)
-apply simp (* [] *)
-apply simp (* ts # tss *)
-apply simp (* [] *)
-apply simp (* t # ts *)
+apply (simp add: ty_denote_ty_lift [where i=0, unfolded substVar_0]) (* TyAll *)
+apply (simp add: ty_denote_ty_lift [where i=0, unfolded substVar_0]) (* TyLam *)
+apply (simp add: ty_denote_ty_lift [where i=0, unfolded substVar_0]) (* TyFix *)
+apply (simp add: cons_subst_conv_map args_subst_conv_map)
+apply (simp add: list_all_iff cong: map_cong)
 done
 
 lemma step_ty_denote:
-  "step t u \<Longrightarrow> ty_denote \<sigma> t = ty_denote \<sigma> u"
+  "step t t' \<Longrightarrow> ty_denote \<sigma> t = ty_denote \<sigma> t'"
 apply (induct arbitrary: \<sigma> set: step)
 txt "unfold"
 apply (simp add: ty_denote_ty_subst substVar_0)
 apply (subst fix_eq, simp)
 txt "beta"
 apply (simp add: ty_denote_ty_subst substVar_0)
-txt "etc"
-apply simp_all
+apply simp (* TyVar *)
+apply simp (* TyBase *)
+apply simp (* TyApp *)
+apply simp (* TyAll *)
+apply simp (* TyLam *)
+apply simp (* TyFix *)
 txt "TyData"
+apply simp
 apply (rule cfun_arg_cong)
-apply (erule list_all2_induct, simp)
-apply (erule list_all2_induct, simp, simp)
+apply (erule list_all2_induct, simp_all)
+apply (erule list_all2_induct, simp_all)
 done
 
 lemma steps_ty_denote:
-  "steps t u \<Longrightarrow> ty_denote \<sigma> t = ty_denote \<sigma> u"
-apply (induct set: steps)
-apply simp (* Why does "rule refl" fail? *)
-apply (auto dest: step_ty_denote)
-done
+  "steps t t' \<Longrightarrow> ty_denote \<sigma> t = ty_denote \<sigma> t'"
+by (induct set: steps, auto dest: step_ty_denote)
 
-lemma conv_ty_denote:
-  "conv t u \<Longrightarrow> ty_denote \<sigma> t = ty_denote \<sigma> u"
-apply (induct set: conv)
-apply (erule trans [OF steps_ty_denote])
-apply (erule sym [OF steps_ty_denote])
-done
+lemma conv_imp_ty_denote:
+  "conv t1 t2 \<Longrightarrow> ty_denote \<sigma> t1 = ty_denote \<sigma> t2"
+by (induct set: conv, simp add: steps_ty_denote)
 
 end
